lowercase r

PhysLean/Relativity/Lorentz/Group/Restricted.lean
@@ -27,7 +27,7 @@ open minkowskiMatrix
 
 /-- The restricted Lorentz group comprises the proper and orthochronous elements of the
 Lorentz group. -/
-def Restricted (d : ℕ) : Subgroup (LorentzGroup d) where
+def restricted (d : ℕ) : Subgroup (LorentzGroup d) where
   carrier := { Λ : LorentzGroup d | IsProper Λ ∧ IsOrthochronous Λ }
   one_mem' := ⟨
     by rw [IsProper]; exact det_one,
@@ -49,7 +49,7 @@ def Restricted (d : ℕ) : Subgroup (LorentzGroup d) where
       by rw [IsOrthochronous, inv_eq_dual, h_dual]; exact Λ_ortho⟩
 
 /-- The restricted Lorentz group is a normal subgroup of the Lorentz group. -/
-lemma restricted_normal_subgroup {d : ℕ} : (Restricted d).Normal := by
+lemma restricted_normal_subgroup {d : ℕ} : (restricted d).Normal := by
   have h_proper {Λ P : LorentzGroup d} (hP : IsProper P) : IsProper (Λ * P * Λ⁻¹) := by
     simp only [IsProper, lorentzGroupIsGroup_mul_coe, det_mul]
     rw [hP, mul_one, ← det_mul, coe_inv, mul_inv_of_invertible, det_one]
